Examples.lean
@@ -1,0 +1,119 @@
+import PBN
+
+theorem a_proof_of_negation (a : Prop) :
+    a → ¬¬ a :=
+  by
+    rw [Not]
+    rw [Not]
+    intro ha
+    intro hna
+    apply hna
+    exact ha
+
+theorem a_proof_of_negation2 (a : Prop) :
+    a → ¬¬ a :=
+  by
+    rw [Not]
+    rw [Not]
+    intro ha
+    intro hna
+    sorry
+    --navigate
+
+  theorem test (a b c d m : Prop) (f : a → b) (h : c → d) (i : b → d) (j: m → d) (k : a → b → c) (M : b → a) (bb : b):
+    (b → c) :=
+  by
+    --navigate
+    --printANDOR
+    sorry
+
+  def test2 (a : Prop) (b : Prop) (c : Prop) (d : Prop) (m : Prop) (f : Int → String) (f2 : Int → String)  (g : a → Int) (h : c → d) (i : b → d) (j: m → d) (k : a → b → c) (bb : b):
+    (a → String) :=
+  by
+    intro ha
+    apply f
+    have x := i ?bbbb
+    . sorry
+    sorry
+    --navigate
+
+  theorem testingg (c d e : Prop) (g : d → e → c) (hd : d) (he : e) :
+    c :=
+  by
+    have x := g hd he
+    --navigate
+    sorry
+
+  theorem testinggg (a b c d e : Prop) (g : a → b → d → e → c) (hd : d) (he : e) :
+    e → c :=
+  by
+    --navigate
+    sorry
+
+  theorem testingggg (a b c : Prop) (ab : a → b) (bc : b → c):
+    a → c :=
+  by
+    intro ha
+    --have x := ab ha
+    --navigate
+    sorry
+
+def testinggggg (a b c d f : Prop) (hb : b) (hc : c) (bca : b → c → a) (cda : c → d → a):
+    a :=
+  by
+    navigate
+
+    --have ha := bca hb hc
+    printANDOR
+    navbottomup
+    --have x := bca hb
+    sorry
+
+  theorem testd (a b c d m : Prop) (f : a → b) (k : a → b → c) :
+    c :=
+  by
+    --navigate
+    --printANDOR
+    --navbottomup
+    sorry
+
+theorem testt (a b c d e x y z : Prop) (f : b → c → a) (g : c → d → a) (h : e → x → z → b) (i : z → y → b)
+-- (he : e) (hx : x) (hy : y) (hz : z)
+:
+    a :=
+  by
+    --navigate
+    have hx: x := sorry
+    have h' he hz := h he hx hz
+
+    have he: e := sorry
+    have h' := h he
+
+    all_goals have hb: b := ?b
+    all_goals have hx: x := sorry
+    all_goals have hz: z := sorry
+    case b => grind
+
+      -- apply h <;> trivial
+
+
+
+
+    printANDOR
+    navbottomup
+    sorry
+
+theorem testtt (a b c d e x y z : Prop) (f : b → c → a) (g : c → d → a) (k : e → x → z → b) (i : z → y → b) (he : e) (ea : e → a) (hy : y):
+    a :=
+  by
+
+    navigate
+    printANDOR
+    navbottomup
+    have j : y := ?b
+
+    navhave h e
+    . apply ea
+      exact h
+    . exact hy
+    . exact he
