PBN/Providers.lean
@@ -1,0 +1,184 @@
+-- tactics over AND-OR trees and graphs
+
+import Lean
+import Std.Data.HashMap
+import PBN.AndOr
+
+open Std
+open Lean Lean.Elab.Tactic
+open Lean Elab Tactic Meta
+
+
+set_option autoImplicit false
+set_option tactic.hygienic false
+
+def navTopDown (node : AndOrStructure LocalDecl) : TacticM Unit := do
+  match node with
+  | AndOrStructure.root _ children =>
+    -- present "apply" for each rule
+    for rule in children do
+      let r ← getNodeExpr rule
+      logInfo m!"apply {r}"
+  | AndOrStructure.or _ _ => return
+  | AndOrStructure.and _ _ => return
+  | AndOrStructure.leaf _ => return
+
+  def navAllPossibilities (node : AndOrStructure LocalDecl) : TacticM Unit := do
+  match node with
+
+  | AndOrStructure.root _ children =>
+    -- present "apply" for each rule
+    for rule in children do
+      let r ← getNodeExpr rule
+      logInfo m!"apply {r}"
+    for rule in children do
+      navAllPossibilities rule
+
+  | AndOrStructure.or _ children =>
+    for rule in children do
+      navAllPossibilities rule
+
+  | AndOrStructure.and v children =>
+    let mut args := m!""
+    if children.length > 0 then
+      for or in children do
+        let o ← getNodeExpr or
+        args := args ++ m!" {o}"
+      logInfo m!"have _ := {v.userName}{args}"
+
+    for or in children do
+      navAllPossibilities or
+
+  | AndOrStructure.leaf _ => return
+
+def printAndOr : TacticM Unit :=
+  withMainContext do
+    let lctx ← getLCtx
+    let mainTarget ← getMainTarget
+    let tree ← buildAndOrTree lctx mainTarget AndORNodeType.ROOT []
+
+    let emptyGraph : ANDORGraph := { edges := [], nodeMap := {}, root := "", andMap := {}}
+    let graph ← toGraph tree emptyGraph []
+
+    traverse_graph graph graph.root []
+
+elab "printANDOR" : tactic => do
+   printAndOr
+
+-- for now get offered all possible applications
+def Navigate : TacticM Unit :=
+  withMainContext do
+    let lctx ← getLCtx
+    let mainTarget ← getMainTarget
+    let tree ← buildAndOrTree lctx mainTarget AndORNodeType.ROOT []
+    navTopDown tree
+    --navAllPossibilities tree
+
+elab "navigate" : tactic => do
+  Navigate
+
+def NavBottomUp : TacticM Unit :=
+  withMainContext do
+    let lctx ← getLCtx
+    let mainTarget ← getMainTarget
+    let tree ← buildAndOrTree lctx mainTarget AndORNodeType.ROOT []
+    let emptyGraph : ANDORGraph := { edges := [], nodeMap := {}, root := "", andMap := {}}
+    let graph ← toGraph tree emptyGraph []
+
+    -- rule map : rule (string version) -> are all args axiomotized?
+    let mut ruleMap : HashMap String Bool := {}
+    let mut argMap : HashMap String Bool := {}
+    -- for all nodes
+    for (_, node) in graph.nodeMap do
+      match node with
+      | Node.AND _ c p _ =>
+        -- if it is a leaf
+        if List.length c == 0 then
+
+          -- if it is AND, record which goal is true and which rule that goal is a child of
+          for goal in p do
+            argMap := argMap.insert goal true
+            let goalnode := graph.nodeMap.get? goal
+            match goalnode with
+            | Node.OR _ _ p2 =>
+              for rule in p2 do
+                -- if rule in rule map, do nothing
+                -- if rule not in rule map, add rule -> true
+                if !ruleMap.contains rule then
+                  ruleMap := ruleMap.insert rule true
+            | _ => continue
+
+      | Node.OR s c p =>
+        -- if it is a leaf
+        if List.length c == 0 then
+          -- if it is an OR, record which goal is not true and which rule it is a child of
+          argMap := argMap.insert s false
+          for rule in p do
+            -- add rule -> false to rule map no matter what
+            ruleMap := ruleMap.insert rule false
+
+    -- for rule in rule map, if true, offer to "have". If false offer "provide" for all non-axiomotized arguments
+    for (rule, b) in ruleMap do
+      let ruleNode := graph.nodeMap.get? rule
+      match ruleNode with
+      | Node.AND s _ _ x =>
+        --logInfo m!"getargs and map: "
+       -- for (a, b) in graph.andMap do
+         -- logInfo m!"{a}, {b}"
+
+        match b with
+        | true =>
+          let mut args ← getArgs x graph.andMap
+          args := List.reverse args
+          let argString := String.intercalate " " args
+          logInfo m!"have _ := {s} {argString}"
+        | false =>
+          let mut args ← getArgsRaw x
+          for arg in args do
+          let arg_status := argMap.get? arg
+          match arg_status with
+          | true => continue
+          | false => logInfo m!"provide {arg}"
+          | _ => continue--logInfo m!"provide {arg}"
+      | _ => continue
+
+elab "navbottomup" : tactic => do
+  NavBottomUp
+
+def navHave (toHave : Expr) (h : Ident) (mvar : Expr) : TacticM (List MVarId) := do
+  let g ← getMainGoal
+  logInfo m!"goal: {g}"
+  let lctx ← getLCtx
+  let name := lctx.getUnusedName `h
+  let g ← g.assert name toHave mvar
+  let (_, g') ← g.intro h.getId
+  return [g']
+
+-- "super have"
+-- new goal
+-- residual context/residual graph
+-- throughout all contexts
+elab "navhave" h:ident t:term : tactic => do
+  let e ← elabTerm t none
+  let mvar ← mkFreshExprMVar (e)
+  let goals ← getGoals
+  let mut new_goals : List MVarId := []
+  for goal in goals do
+    let get_goal ← goal.withContext do
+      navHave e h mvar
+    new_goals := new_goals ++ get_goal
+  new_goals := new_goals ++ [mvar.mvarId!]
+  replaceMainGoal new_goals
+
+  -- for each context
+    -- build and-or graph
+    -- prune the stuff that is only a descendant of t- get back a list of hypotheses to delete from the context
+
+    -- w = t
+    -- while having w satisfies some rule(s),
+      -- prune stuff below the rule and any alternate rules to prove the new goal(s)
+      -- w = new goal(s)
+    -- get back another list of hypotheses to delete from context
+
+
+-- next- essential things, order
