out_of_date/Basic.lean
@@ -1,0 +1,667 @@
+import Lean
+import Std.Data.HashMap
+
+open Std
+open Lean Lean.Elab.Tactic
+open Lean Elab Tactic Meta
+
+set_option autoImplicit false
+set_option tactic.hygienic false
+
+inductive Node
+  | OR (expr: String) (children : List String) (parents : List String)
+  | AND (name: String) (children : List String) (parents : List String) (expression : Expr)
+
+structure Edge where
+  parent : String
+  child : String
+
+structure ANDORGraph where
+  root : String
+  edges : List Edge
+  nodeMap : HashMap String Node
+  andMap : HashMap String String -- map rule exp to name
+
+inductive AndORNodeType
+  | ROOT
+  | OR
+
+inductive AndOrStructure (V : Type)
+  | leaf (v : V)
+  | root (v : Expr) (children : List (AndOrStructure V))
+  | or   (v : Expr) (children : List (AndOrStructure V))
+  | and  (v : V) (children : List (AndOrStructure V))
+
+def toGraph (tree: AndOrStructure LocalDecl) (graph_in : ANDORGraph) (parent_in : List String) : TacticM ANDORGraph := do
+  let mut edges := graph_in.edges
+  let mut nodeMap := graph_in.nodeMap
+  let mut root := graph_in.root
+  let mut parent := parent_in
+  let mut andMap := graph_in.andMap
+
+  --logInfo m!"top and map: "
+  --for (a, b) in andMap do
+    --logInfo m!"{a}, {b}"
+
+  match tree with
+  | AndOrStructure.root v children => do
+
+    --let mut string_rep ← m!"{v}".toString
+    let fmt ← PrettyPrinter.ppExpr v
+    let string_rep := fmt.pretty
+
+    let mut node_children : List String := []
+
+    -- add edges to children
+    for child in children do
+
+      match child with
+      | AndOrStructure.and v c =>
+        let child_string := s!"{v.userName}"
+        let edge : Edge := { parent := string_rep, child := child_string}
+        node_children := child_string :: node_children
+        edges := edge :: edges
+        let graph_arg : ANDORGraph := { edges := edges, nodeMap := nodeMap, root := root, andMap := andMap}
+        let new_graph ← toGraph child graph_arg [string_rep]
+        edges := new_graph.edges
+        nodeMap := new_graph.nodeMap
+        andMap := new_graph.andMap
+
+      | AndOrStructure.leaf v =>
+        let child_string := s!"{v.userName}"
+        let edge : Edge := { parent := string_rep, child := child_string }
+        edges := edge :: edges
+        node_children := child_string :: node_children
+        let graph_arg : ANDORGraph := { edges := edges, nodeMap := nodeMap, root := root, andMap := andMap}
+        let new_graph ← toGraph child graph_arg [string_rep]
+        edges := new_graph.edges
+        nodeMap := new_graph.nodeMap
+        andMap := new_graph.andMap
+
+      | _ => continue
+
+    -- replace node but with more parents if already exists
+    let node_maybe := nodeMap.get? string_rep
+
+    match node_maybe with
+    | Node.OR e c p => parent := p ++ parent
+    | Node.AND e c p x=> parent := p ++ parent
+    | _ => parent := parent
+
+    let node := Node.OR string_rep node_children parent
+    nodeMap := nodeMap.insert string_rep node
+    let ret_graph : ANDORGraph := { edges := edges, nodeMap := nodeMap, root := string_rep, andMap := andMap}
+    return ret_graph
+
+  | AndOrStructure.or v children => do
+    --let string_rep := s!"{v}"
+    let fmt ← PrettyPrinter.ppExpr v
+    let string_rep := fmt.pretty
+    let mut node_children : List String := []
+
+    -- add edges to children
+    for child in children do
+      match child with
+      | AndOrStructure.and v c =>
+        let child_string := s!"{v.userName}"
+        let edge : Edge := { parent := string_rep, child := child_string }
+        edges := edge :: edges
+        node_children := child_string :: node_children
+        let graph_arg : ANDORGraph := { edges := edges, nodeMap := nodeMap, root := root, andMap := andMap}
+        let new_graph ← toGraph child graph_arg [string_rep]
+        edges := new_graph.edges
+        nodeMap := new_graph.nodeMap
+        andMap := new_graph.andMap
+
+      | AndOrStructure.leaf v =>
+        let child_string := s!"{v.userName}"
+        let edge : Edge := { parent := string_rep, child := child_string }
+        edges := edge :: edges
+        node_children := child_string :: node_children
+        let graph_arg : ANDORGraph := { edges := edges, nodeMap := nodeMap, root := root, andMap := andMap}
+        let new_graph ← toGraph child graph_arg [string_rep]
+        edges := new_graph.edges
+        nodeMap := new_graph.nodeMap
+        andMap := new_graph.andMap
+
+      | _ => continue
+
+    -- replace node but with more parents if already exists
+    let node_maybe := nodeMap.get? string_rep
+
+    match node_maybe with
+    | Node.OR e c p => parent := p ++ parent
+    | Node.AND e c p x => parent := p ++ parent
+    | _ => parent := parent
+
+    -- make node
+    let node := Node.OR string_rep node_children parent
+    nodeMap := nodeMap.insert string_rep node
+    let ret_graph : ANDORGraph := { edges := edges, nodeMap := nodeMap, root := root, andMap := andMap }
+    return ret_graph
+
+  | AndOrStructure.and v children => do
+    -- make node
+    let ld ← inferType v.toExpr
+    let string_rep := s!"{v.userName}"
+
+    let ldfmt ← PrettyPrinter.ppExpr ld
+    let ldString := ldfmt.pretty
+
+    andMap := andMap.insert ldString string_rep
+
+    --logInfo m!"andMap: {m!"{ld}"}, {string_rep}"
+
+    let mut node_children : List String := []
+    -- add edges to children
+    for child in children do
+      match child with
+      | AndOrStructure.or v _ =>
+        --let child_string := s!"{v}"
+        let fmtchild ← PrettyPrinter.ppExpr v
+        let child_string := fmtchild.pretty
+        let edge : Edge := { parent := string_rep, child := child_string }
+        edges := edge :: edges
+        node_children := child_string :: node_children
+        let graph_arg : ANDORGraph := { edges := edges, nodeMap := nodeMap, root := root, andMap := andMap}
+        let new_graph ← toGraph child graph_arg [string_rep]
+        edges := new_graph.edges
+        nodeMap := new_graph.nodeMap
+        andMap := new_graph.andMap
+
+      | _ => continue
+
+    -- replace node but with more parents if already exists
+    let node_maybe := nodeMap.get? string_rep
+
+    match node_maybe with
+    | Node.OR e c p => parent := p ++ parent
+    | Node.AND e c p x => parent := p ++ parent
+    | _ => parent := parent
+
+
+    let node := Node.AND string_rep node_children parent ld
+    nodeMap := nodeMap.insert string_rep node
+    let ret_graph : ANDORGraph := { edges := edges, nodeMap := nodeMap, root := root, andMap := andMap }
+    return ret_graph
+
+  | AndOrStructure.leaf v => do
+    -- make node
+    let ld ← inferType v.toExpr
+    let string_rep := s!"{v.userName}"
+
+    let ldfmt ← PrettyPrinter.ppExpr ld
+    let ldString := ldfmt.pretty
+
+    andMap := andMap.insert ldString string_rep
+    --logInfo m!"andMap: {m!"{ld}"}, {string_rep}"
+
+    -- replace node but with more parents if already exists
+    let node_maybe := nodeMap.get? string_rep
+
+    match node_maybe with
+    | Node.OR e c p => parent := p ++ parent
+    | Node.AND e c p x => parent := p ++ parent
+    | _ => parent := parent
+
+
+    let node := Node.AND string_rep [] parent ld
+    nodeMap := nodeMap.insert string_rep node
+
+    let ret_graph : ANDORGraph := { edges := edges, nodeMap := nodeMap, root := root, andMap := andMap }
+    return ret_graph
+
+partial def traverse_graph (graph : ANDORGraph) (node_string : String) (seen_in : List String) : TacticM Unit := do
+  if node_string ∈ seen_in then
+    return
+
+  let seen := node_string :: seen_in
+
+  let nodeMap := graph.nodeMap
+
+  let node : Option Node := nodeMap.get? node_string
+
+  match node with
+  | Node.OR rep children p =>
+    logInfo m!"OR: {rep}, children: {children}, parents : {p}"
+    for child in children do
+      traverse_graph graph child seen
+  | Node.AND rep children p x =>
+    logInfo m!"AND: {rep}, children: {children}, parents : {p}"
+    for child in children do
+      traverse_graph graph child seen
+  | _ => return
+
+
+def PrintSubtree (graph: AndOrStructure LocalDecl): TacticM Unit := do
+  match graph with
+  | AndOrStructure.root v children => do
+    logInfo m!"root expr: {v}"
+    for child in children do
+      PrintSubtree child
+  | AndOrStructure.or v children => do
+    logInfo m!"Or: {v}"
+    for child in children do
+      PrintSubtree child
+  | AndOrStructure.and v children => do
+    let name := v.userName
+    let type ← inferType v.toExpr
+    logInfo m!"And: {name} : {type}"
+    for child in children do
+      PrintSubtree child
+  | AndOrStructure.leaf v => do
+    let name := v.userName
+    let type ← inferType v.toExpr
+    logInfo m!"Leaf: {name} : {type}"
+
+def getArgs (e : Expr) (andMap : HashMap String String) : MetaM (List String) := do
+  let mut exp := e
+  let mut args := []
+  while true do
+    exp ← whnf exp
+    match exp with
+    | Expr.forallE _ first body _ =>
+        let fmt ← PrettyPrinter.ppExpr first
+        let string_rep := fmt.pretty
+        let possibleRule := andMap.contains string_rep
+        if possibleRule then
+          let a := andMap.get! string_rep
+          args := [a] ++ args
+        else
+          args := [string_rep] ++ args
+        exp := body
+    | _ => break
+  return args
+
+def getArgsRaw (e : Expr) : MetaM (List String) := do
+  let mut exp := e
+  let mut args := []
+  while true do
+    exp ← whnf exp
+    match exp with
+    | Expr.forallE _ first body _ =>
+        let fmt ← PrettyPrinter.ppExpr first
+        let string_rep := fmt.pretty
+        args := [string_rep] ++ args
+        exp := body
+    | _ => break
+  return args
+
+def dropLeftMost (e : Expr) : MetaM Expr := do
+  let e ← whnf e
+  match e with
+  | Expr.forallE _ _ body _ => return body
+  | _ => return e
+
+  def getFirstArg (e : Expr) : MetaM (List Expr) := do
+  match e with
+  | Expr.forallE _ first _ _ => return [first]
+  | _ => return []
+
+-- for some goal, find rules that could provide it
+partial def buildAndOrTree (lctx : LocalContext) (goal: Expr) (nodeType: AndORNodeType) (seen_in : List String) : MetaM (AndOrStructure LocalDecl):= do
+
+  let fmt ← PrettyPrinter.ppExpr goal
+  let string_rep := fmt.pretty
+
+  if string_rep ∈ seen_in then
+    return AndOrStructure.or goal []
+
+  let mut seen := string_rep :: seen_in
+
+  let mut rules: List (AndOrStructure LocalDecl) := []
+  for ldecl in lctx do
+    let mut args: List Expr := []
+  -- iterate over hypotheses
+    unless ldecl.isImplementationDetail do
+      let mut last : Option Expr := none
+      let mut curr := ← inferType ldecl.toExpr
+
+      -- peel back layer by layer
+       -- if layer is the same as goal, add as rule to get goal
+        --while !curr == mkSort 0 && (last.isNone || !(← isDefEq last.get! curr)) do
+      if (← isDefEq curr goal) then
+          rules := rules ++ [AndOrStructure.leaf ldecl ]
+          continue
+      while true do
+        if curr == mkSort 0 then
+          break
+
+        let mut iterate : Bool ←
+          (match last with
+          | some l => do
+              let eq ← isDefEq l curr
+              pure (¬ eq)
+          | none => pure true)
+
+        if !iterate then
+          break
+
+        if (← isDefEq curr goal) then
+          let mut arg_nodes := []
+          for arg in args do
+
+            -- each arg will be an or subtree
+            let a ← buildAndOrTree lctx arg AndORNodeType.OR seen
+            arg_nodes := a :: arg_nodes
+          rules := rules ++ [AndOrStructure.and ldecl arg_nodes]
+
+        -- else strip a layer
+        last := some curr
+        let arg ← getFirstArg curr
+        args := arg ++ args
+        curr ← dropLeftMost curr
+  match nodeType with
+  | AndORNodeType.ROOT =>
+      let graph : AndOrStructure LocalDecl :=  AndOrStructure.root goal rules
+      return graph
+  | AndORNodeType.OR =>
+      let graph : AndOrStructure LocalDecl :=  AndOrStructure.or goal rules
+      return graph
+
+def getNodeExpr (node : AndOrStructure LocalDecl) : MetaM Expr := do
+  match node with
+  | AndOrStructure.root v children => return v
+  | AndOrStructure.or v children => return v
+  | AndOrStructure.and v children => return v.toExpr
+  | AndOrStructure.leaf v => return v.toExpr
+
+def navTopDown (node : AndOrStructure LocalDecl) : TacticM Unit := do
+  match node with
+  | AndOrStructure.root v children =>
+    -- present "apply" for each rule
+    for rule in children do
+      let r ← getNodeExpr rule
+      logInfo m!"apply {r}"
+  | AndOrStructure.or v children => return
+  | AndOrStructure.and v children => return
+  | AndOrStructure.leaf v => return
+
+  def navAllPossibilities (node : AndOrStructure LocalDecl) : TacticM Unit := do
+  match node with
+
+  | AndOrStructure.root v children =>
+    -- present "apply" for each rule
+    for rule in children do
+      let r ← getNodeExpr rule
+      logInfo m!"apply {r}"
+    for rule in children do
+      navAllPossibilities rule
+
+  | AndOrStructure.or v children =>
+    for rule in children do
+      navAllPossibilities rule
+
+  | AndOrStructure.and v children =>
+    let mut args := m!""
+    if children.length > 0 then
+      for or in children do
+        let o ← getNodeExpr or
+        args := args ++ m!" {o}"
+      logInfo m!"have _ := {v.userName}{args}"
+
+    for or in children do
+      navAllPossibilities or
+
+  | AndOrStructure.leaf v => return
+
+def printAndOr : TacticM Unit :=
+  withMainContext do
+    let lctx ← getLCtx
+    let mainTarget ← getMainTarget
+    let tree ← buildAndOrTree lctx mainTarget AndORNodeType.ROOT []
+
+    let emptyGraph : ANDORGraph := { edges := [], nodeMap := {}, root := "", andMap := {}}
+    let graph ← toGraph tree emptyGraph []
+
+    traverse_graph graph graph.root []
+
+elab "printANDOR" : tactic => do
+   printAndOr
+
+-- for now get offered all possible applications
+def Navigate : TacticM Unit :=
+  withMainContext do
+    let lctx ← getLCtx
+    let mainTarget ← getMainTarget
+    let tree ← buildAndOrTree lctx mainTarget AndORNodeType.ROOT []
+    navTopDown tree
+    --navAllPossibilities tree
+
+elab "navigate" : tactic => do
+  Navigate
+
+def remove_goals (false_set : List String) (graph_in : ANDORGraph) : TacticM ANDORGraph := do
+  let mut edges := []
+  let mut nodeMap := graph_in.nodeMap
+  let root := graph_in.root
+  let mut andMap := graph_in.andMap
+
+  for f in false_set do
+    -- get the goal node
+    let node := nodeMap.get? f
+    match node with
+    | Node.OR s c p =>
+      -- remove the goal node
+      nodeMap := nodeMap.erase f
+      -- remove any edges including the goal node
+      -- remove any parents of the goal node
+      for parent in p do
+
+        -- remove all other children
+        let rule := nodeMap.get? parent
+        match rule with
+        | Node.AND s c p x =>
+          for child in c do
+            nodeMap := nodeMap.erase child
+        | _ => continue
+        -- remove as a child of goals?
+        -- remove from andMap
+        nodeMap := nodeMap.erase parent
+        -- remove from nodeMap
+        andMap := andMap.erase parent
+
+      -- remove the goal node as a parent of any children
+    | _ => continue
+
+
+  let graph_out : ANDORGraph := { edges := edges, nodeMap := nodeMap, root := root, andMap := andMap}
+  return graph_out
+
+
+def NavBottomUp : TacticM Unit :=
+  withMainContext do
+    let lctx ← getLCtx
+    let mainTarget ← getMainTarget
+    let tree ← buildAndOrTree lctx mainTarget AndORNodeType.ROOT []
+    let emptyGraph : ANDORGraph := { edges := [], nodeMap := {}, root := "", andMap := {}}
+    let graph ← toGraph tree emptyGraph []
+
+    -- rule map : rule (string version) -> are all args axiomotized?
+    let mut ruleMap : HashMap String Bool := {}
+    let mut argMap : HashMap String Bool := {}
+    -- for all nodes
+    for (str, node) in graph.nodeMap do
+      match node with
+      | Node.AND s c p x =>
+        -- if it is a leaf
+        if List.length c == 0 then
+
+          -- if it is AND, record which goal is true and which rule that goal is a child of
+          for goal in p do
+            argMap := argMap.insert goal true
+            let goalnode := graph.nodeMap.get? goal
+            match goalnode with
+            | Node.OR s2 c2 p2 =>
+              for rule in p2 do
+                -- if rule in rule map, do nothing
+                -- if rule not in rule map, add rule -> true
+                if !ruleMap.contains rule then
+                  ruleMap := ruleMap.insert rule true
+            | _ => let x := 1
+
+      | Node.OR s c p =>
+        -- if it is a leaf
+        if List.length c == 0 then
+          -- if it is an OR, record which goal is not true and which rule it is a child of
+          argMap := argMap.insert s false
+          for rule in p do
+            -- add rule -> false to rule map no matter what
+            ruleMap := ruleMap.insert rule false
+
+    -- for rule in rule map, if true, offer to "have". If false offer "provide" for all non-axiomotized arguments
+    for (rule, b) in ruleMap do
+      let ruleNode := graph.nodeMap.get? rule
+      match ruleNode with
+      | Node.AND s c p x =>
+        --logInfo m!"getargs and map: "
+       -- for (a, b) in graph.andMap do
+         -- logInfo m!"{a}, {b}"
+
+        match b with
+        | true =>
+          let mut args ← getArgs x graph.andMap
+          args := List.reverse args
+          let argString := String.intercalate " " args
+          logInfo m!"have _ := {s} {argString}"
+        | false =>
+          let mut args ← getArgsRaw x
+          for arg in args do
+          let arg_status := argMap.get? arg
+          match arg_status with
+          | true => continue
+          | false => logInfo m!"provide {arg}"
+          | _ => continue--logInfo m!"provide {arg}"
+      | _ => continue
+
+elab "navbottomup" : tactic => do
+  NavBottomUp
+
+def navHave : TacticM Unit := do
+  sorry
+
+elab "navHave" : tactic => do
+  navHave
+
+
+
+theorem a_proof_of_negation (a : Prop) :
+    a → ¬¬ a :=
+  by
+    rw [Not]
+    rw [Not]
+    intro ha
+    intro hna
+    apply hna
+    exact ha
+
+theorem a_proof_of_negation2 (a : Prop) :
+    a → ¬¬ a :=
+  by
+    rw [Not]
+    rw [Not]
+    intro ha
+    intro hna
+    sorry
+    --navigate
+
+  theorem test (a b c d m : Prop) (f : a → b) (h : c → d) (i : b → d) (j: m → d) (k : a → b → c) (M : b → a) (bb : b):
+    (b → c) :=
+  by
+    --navigate
+    --printANDOR
+    sorry
+
+  def test2 (a : Prop) (b : Prop) (c : Prop) (d : Prop) (m : Prop) (f : Int → String) (f2 : Int → String)  (g : a → Int) (h : c → d) (i : b → d) (j: m → d) (k : a → b → c) (bb : b):
+    (a → String) :=
+  by
+    intro ha
+    apply f
+    --have x := i ?bbbb
+    sorry
+    --navigate
+
+  theorem testingg (c d e : Prop) (g : d → e → c) (hd : d) (he : e) :
+    c :=
+  by
+    have x := g hd he
+    --navigate
+    sorry
+
+  theorem testinggg (a b c d e : Prop) (g : a → b → d → e → c) (hd : d) (he : e) :
+    e → c :=
+  by
+    --navigate
+    sorry
+
+  theorem testingggg (a b c : Prop) (ab : a → b) (bc : b → c):
+    a → c :=
+  by
+    intro ha
+    --have x := ab ha
+    --navigate
+    sorry
+
+def testinggggg (a b c d f : Prop) (hb : b) (hc : c) (bca : b → c → a) (cda : c → d → a):
+    a :=
+  by
+    navigate
+
+    --have ha := bca hb hc
+    printANDOR
+    navbottomup
+    --have x := bca hb
+    sorry
+
+  theorem testd (a b c d m : Prop) (f : a → b) (k : a → b → c) :
+    c :=
+  by
+    --navigate
+    --printANDOR
+    --navbottomup
+    sorry
+
+theorem testt (a b c d e x y z : Prop) (f : b → c → a) (g : c → d → a) (h : e → x → z → b) (i : z → y → b)
+-- (he : e) (hx : x) (hy : y) (hz : z)
+:
+    a :=
+  by
+    --navigate
+    have hx: x := sorry
+    have h' he hz := h he hx hz
+
+
+
+    have he: e := sorry
+    have h' := h he
+
+    all_goals have hb: b := ?b
+    all_goals have hx: x := sorry
+    all_goals have hz: z := sorry
+    case b => grind
+
+      -- apply h <;> trivial
+
+
+
+
+    printANDOR
+    navbottomup
+    sorry
+
+theorem testtt (a b c d e x y z : Prop) (f : b → c → a) (g : c → d → a) (h : e → x → z → b) (i : z → y → b) (he : e):
+    a :=
+  by
+
+    navigate
+    printANDOR
+    navbottomup
+    sorry
+
+
+-- "super have"
+  -- new goal
+  -- residual context/residual graph
+  -- throughout all contexts
+
+-- next- essential things, order
